Examples/StellarConsensus/SCP.lean
@@ -3,41 +3,51 @@ import Examples.StellarConsensus.SCPTheory
 
 -- adapted from [SCP.ivy](https://github.com/stellar/scp-proofs/blob/3e0428acc78e598a227a866b99fe0b3ad4582914/SCP.ivy)
 
-/-
-  NOTE: For now we do not prove liveness property in Veil, so we only
-  adapt the proof for `intertwined_safe`.
--/
 
 /-- This type class bundles the properties abstracted from the concrete model
     of SCP, which will be used in the subsequent verification.
     In the Ivy spec, they appear as `trusted` properties (assumptions). -/
-class SCP.Background (node : outParam Type) (nset : outParam Type) where
+class SCP.FBQS_Safety (node : outParam Type) (nset : outParam Type) where
   well_behaved : node → Prop
   intertwined : node → Prop
   intact : node → Prop
   member : node → nset → Prop
   is_quorum : nset → Prop
-  blocks_slices : nset → node → Prop
+  slice_blocking : nset → node → Prop
 
+  -- Basic properties of node sets
   axiom_0 : ∀ (n : node), intact n → intertwined n
   axiom_1 : ∀ (n : node), intertwined n → well_behaved n
+  -- Needed for safety
   qi_intertwined : ∀ (q1 q2 : nset),
     (∃ (n1 : node), intertwined n1 ∧ is_quorum q1 ∧ member n1 q1) ∧
     (∃ (n2 : node), intertwined n2 ∧ is_quorum q2 ∧ member n2 q2) →
     ∃ (n3 : node), well_behaved n3 ∧ member n3 q1 ∧ member n3 q2
 
+class SCP.FBQS (node : outParam Type) (nset : outParam Type) extends SCP.FBQS_Safety node nset where
+  -- Needed for liveness (we keep these separate for decidability)
+  qi_intact : ∀ (q1 q2 : nset),
+    (∃ (n1 : node), intact n1 ∧ is_quorum q1 ∧ member n1 q1) ∧
+    (∃ (n2 : node), intact n2 ∧ is_quorum q2 ∧ member n2 q2) →
+    ∃ (n3 : node), intact n3 ∧ member n3 q1 ∧ member n3 q2
+  slice_blocks_ne : ∀ (s : nset),
+    (∃ (n : node), intact n ∧ slice_blocking s n) →
+    ∃ (n2 : node), member n2 s ∧ intact n2
+  intact_is_quorum :
+    ∃ (q : nset), (∀ (n : node), member n q ↔ intact n) ∧ is_quorum q
+
 /-- Given a concrete system model `FBA.System`, fix the intertwined set `S` and
     the intact set `I ⊆ S` to consider, all abstracted properties can be satisfied. -/
-def one_such_Background (node : Type) [fba : FBA.System node]
-    (I : Set node) (_hI : FBA.intact (inst := fba) I)
+def one_such_FBQS (node : Type) [fba : FBA.System node]
+    (I : Set node) (hI : FBA.intact (inst := fba) I)
     (S : Set node) (hS : FBA.intertwined (inst := fba) S)
-    (hIS : I ⊆ S) : SCP.Background node (Set node) where
+    (hIS : I ⊆ S) : SCP.FBQS node (Set node) where
   well_behaved n := n ∈ fba.W
   intertwined n := n ∈ S
   intact n := n ∈ I
   member n s := n ∈ s
   is_quorum := FBA.quorum (inst := fba)
-  blocks_slices := FBA.blocks_slices (inst := fba)
+  slice_blocking := FBA.slice_blocking (inst := fba)
 
   axiom_0 := by assumption
   axiom_1 := by
@@ -60,6 +70,26 @@ def one_such_Background (node : Type) [fba : FBA.System node]
     apply And.intro
     · apply FBA.intertwined_node_is_well_behaved <;> assumption
     · assumption
+  qi_intact := by
+    simp
+    intro q1 q2 n1 hn1I hq1 hn1q1 n2 hn2I hq2 hn2q2
+    have hinter := hI.q_inter q1 q2
+      (FBA.quorum_after_proj (inst := fba) q1 I hq1)
+      (FBA.quorum_after_proj (inst := fba) q2 I hq2)
+    repeat rw [FBA.set_ne_empty_iff_exists_mem] at hinter
+    simp only [Set.mem_inter_iff, forall_exists_index, and_imp] at hinter
+    specialize hinter n1 hn1q1 hn1I n2 hn2q2 hn2I
+    rcases hinter with ⟨n3, ⟨hn3q1, hn3q2⟩, hn3I⟩
+    exact ⟨n3, hn3I, hn3q1, hn3q2⟩
+  slice_blocks_ne := by
+    intro s hs
+    rcases hs with ⟨n, hnI, hblocks⟩
+    have h := FBA.slice_blocks_ne (inst := fba) n s I hI hnI hblocks
+    rw [FBA.set_ne_empty_iff_exists_mem] at h
+    rcases h with ⟨n2, hn2s, hn2I⟩
+    exact ⟨n2, hn2s, hn2I⟩
+  intact_is_quorum := by
+    exact ⟨I, by simp, hI.q_avail⟩
 
 veil module SCP
 
@@ -72,9 +102,9 @@ type ballot
    but neither `next` nor `prev` appears in the protocol or any invariant.
    So here we model `ballot` as simply a `TotalOrderWithMinimum`. -/
 instantiate tot : TotalOrderWithMinimum ballot
-instantiate bg : Background node nset
+instantiate bg : FBQS_Safety node nset
 
-open Background
+open FBQS_Safety
 
 -- Parts for the protocol.
 relation voted_prepared (N : node) (B : ballot) (V : value)
@@ -93,21 +123,6 @@ relation received_vote_commit (N1 : node) (N2 : node) (B : ballot) (V : value)
 relation received_accept_commit (N1 : node) (N2 : node) (B : ballot) (V : value)
 
 #gen_state
-
--- NOTE: the following seem to be unnecessary for proving the safety.
-/-
-assumption [qi_intact]
-  ∀ (q1 q2 : nset),
-    (∃ (n1 : node), intact n1 ∧ is_quorum q1 ∧ member n1 q1) ∧
-    (∃ (n2 : node), intact n2 ∧ is_quorum q2 ∧ member n2 q2) →
-    ∃ (n3 : node), intact n3 ∧ member n3 q1 ∧ member n3 q2
-
-assumption [slice_blocks_ne]
-  ∀ (s : nset), (∃ (n : node), intact n ∧ blocks_slices s n) → ∃ (n2 : node), member n2 s ∧ intact n2
-
-assumption [intact_is_quorum]
-  ∃ (q : nset), (∀ (n : node), member n q ↔ intact n) ∧ is_quorum q
--/
 
 after_init {
   voted_prepared N B V := false
@@ -162,7 +177,7 @@ action receive_accept_prepare (na nb : node) (b : ballot) (v : value) {
       voted_committed na b v := true
   if ((∃ Q, is_quorum Q ∧ member na Q ∧
         (∀ N, member N Q → (received_vote_prepare na N b v ∨ received_accept_prepare na N b v)))
-      ∨ (∃ S, blocks_slices S na ∧ (∀ N, member N S → received_accept_prepare na N b v)))
+      ∨ (∃ S, slice_blocking S na ∧ (∀ N, member N S → received_accept_prepare na N b v)))
     ∧ (∀ B V, ¬ (accepted_committed na B V ∧ tot.lt B b ∧ V ≠ v))
     ∧ (∀ V, ¬ accepted_prepared na b V) then
     accepted_prepared na b v := true
@@ -187,7 +202,7 @@ action receive_accept_commit (na nb : node) (b : ballot) (v : value) {
     confirmed_committed na b v := true
   if ((∃ Q, is_quorum Q ∧ member na Q ∧
         (∀ N, member N Q → (received_vote_commit na N b v ∨ received_accept_commit na N b v)))
-      ∨ (∃ S, blocks_slices S na ∧ (∀ N, member N S → received_accept_commit na N b v)))
+      ∨ (∃ S, slice_blocking S na ∧ (∀ N, member N S → received_accept_commit na N b v)))
     ∧ (∀ B V, ¬ (accepted_prepared na B V ∧ tot.lt b B ∧ V ≠ v))
     ∧ (∀ V, ¬ accepted_committed na b V)
     ∧ confirmed_prepared na b v then
@@ -241,6 +256,6 @@ invariant ∀ N B V1 V2,
 
 #gen_spec
 
-#time #check_invariants
+#check_invariants
 
 end SCP
